src/Cvm_Monad.v
@@ -101,11 +101,46 @@ Definition fwd_asp (fwd:FWD) (bs:BS) (e:EvC) (p:Plc) (ps:ASP_PARAMS): EvC :=
   | KEEP => e
   end.
 
+(** * Stub for invoking external ASP procedures.  
+      Extracted code should not need to use the Plc or Event_ID parameters 
+      (those can be erased upon extraction). *)
+Definition do_asp (params :ASP_PARAMS) (e:RawEv) (mpl:Plc) (x:Event_ID) (ac : AM_Config) : ResultT BS DispatcherErrors :=
+  (ac.(aspCb) params mpl (encodeEvRaw e) e).
+
+  Check dispatch_error.
+  Locate dispatch_error.
+
+  Print ASP_PARAMS.
+
+Definition do_ext_asp (ps:ASP_PARAMS) (ac: AM_Config) (e:RawEv) : ResultT BS DispatcherErrors := 
+  match ps with 
+  | asp_paramsC i _ _ _ => 
+
+  let asp_uuid_res : ResultT UUID DispatcherErrors := ac.(ext_aspCb) i in
+    match asp_uuid_res with 
+    | resultC uuid => 
+        match doAsp_uuid uuid e with
+        | resultC v => resultC v
+        | errC (messageLift msg) => errC (Runtime msg)
+        end
+    | errC e => errC e
+    end
+
+  end.
+
 Definition do_asp' (params :ASP_PARAMS) (e:RawEv) (mpl:Plc) (x:Event_ID) : CVM BS :=
   ac <- get_CVM_amConfig  ;;
   match (do_asp params e mpl x ac) with
-  | resultC r => ret r
-  | errC e => failm (dispatch_error e)
+  | resultC v => ret v
+  | errC err => 
+    match err with 
+    | Unavailable => 
+      match (do_ext_asp params ac e) with 
+      | resultC v => ret v
+      | errC err' => failm (dispatch_error err') 
+      end
+    | Runtime s => failm (dispatch_error (Runtime s))
+    end
   end.
 
 (* Simulates invoking an arbitrary ASP.  Tags the event, builds and returns 
@@ -191,6 +226,18 @@ Definition check_cvm_policy (t:Term) (pTo:Plc) (et:Evidence) : CVM unit :=
     | false => failm (dispatch_error (Runtime errStr_disclosePolicy))
     end.
 
+
+Definition do_remote (t:Term) (pTo:Plc) (e:EvC) (ac: AM_Config) : ResultT RawEv DispatcherErrors := 
+  let remote_uuid_res : ResultT UUID DispatcherErrors := ac.(plcCb) pTo in
+    match remote_uuid_res with 
+    | resultC uuid => 
+        match doRemote_uuid t uuid (get_bits e) with
+        | resultC v => resultC v
+        | errC (messageLift msg) => errC (Runtime msg)
+        end
+    | errC e => errC e
+    end.
+
 Definition doRemote_session' (t:Term) (pTo:Plc) (e:EvC) : CVM EvC := 
   check_cvm_policy t pTo (get_et e) ;;
   ac <- get_CVM_amConfig ;;
@@ -221,6 +268,12 @@ Definition join_seq (e1:EvC) (e2:EvC): CVM unit :=
 (* Primitive monadic parallel CVM thread primitives 
    (some rely on Admitted IO Stubs). *)
 
+Definition do_start_par_thread (loc:Loc) (t:Core_Term) (e:RawEv) : CVM unit :=
+  ret tt.
+
+Definition do_wait_par_thread (loc:Loc) (t:Core_Term) (p:Plc) (e:EvC) : CVM EvC :=
+  ret (parallel_vm_thread loc t p e).
+
 Definition start_par_thread (loc:Loc) (t:Core_Term) (e:EvC) : CVM unit :=
   p <- get_pl ;;
   do_start_par_thread loc t (get_bits e) ;;
@@ -239,6 +292,7 @@ Ltac monad_unfold :=
   do_prim,
   invoke_ASP,
   do_asp',
+  do_ext_asp,
   do_asp,
   clearEv,
   copyEv,
